Slide Dependence

Slicing.dfy
@@ -3,7 +3,7 @@ include "Util.dfy"
 include "PDG.dfy"
 include "SlideDG.dfy"
 
-method ComputeSlice(S: Statement, V: set<Variable>) returns (S_V: set<Slide>)
+method {:verify false}ComputeSlice(S: Statement, V: set<Variable>) returns (S_V: set<Slide>)
 {
 	var cfg := ComputeCFG(S);
 	var pdgN, pdgE := ComputePDG(S, cfg); // TODO: Change to PDG
@@ -21,7 +21,7 @@ method ComputeSlice(S: Statement, V: set<Variable>) returns (S_V: set<Slide>)
 	}
 }
 
-method finalDefSlides(slideDG: SlideDG, cfg: CFG, V: set<Variable>) returns (S_V: set<Slide>)
+method {:verify false}finalDefSlides(slideDG: SlideDG, cfg: CFG, V: set<Variable>) returns (S_V: set<Slide>)
 {
 	S_V := {};
 	var copyV := V;
@@ -36,12 +36,11 @@ method finalDefSlides(slideDG: SlideDG, cfg: CFG, V: set<Variable>) returns (S_V
 	}
 }
 
-method finalDefSlidesOfVariable(slideDG: SlideDG, cfg: CFG, v: Variable) returns (Sv: set<Slide>)
+method {:verify false}finalDefSlidesOfVariable(slideDG: SlideDG, cfg: CFG, v: Variable) returns (Sv: set<Slide>)
 {
 	Sv := {};
-	var vDefNodes := findDefNodes(slideDG.0, slideDG.1, v);
-	// find all def nodes of v in slideDG
-
+	var vDefNodes := findDefNodes(slideDG.0, slideDG.1, v); // find all def nodes of v in slideDG
+	
 	while (|vDefNodes| > 0)
 	{
 		var vDefNode :| vDefNode in vDefNodes;
@@ -52,7 +51,7 @@ method finalDefSlidesOfVariable(slideDG: SlideDG, cfg: CFG, v: Variable) returns
 			case Node(l) =>
 				var cfgNode := CFGNode.Node(l);
 				var pathsToExit := findAllPathsToExit(slideDG.0, cfg, [cfgNode], {}); // foreach node - find all paths to exit (in cfg) - seq of cfg nodes
-				var res := isFinalDefSlide(pathsToExit, vDefNode /* or cfgNode */, v);		 // check if there is at least one path that it's only def is in the source node
+				var res := isFinalDefSlide(slideDG.0, pathsToExit, vDefNode);	      // check if there is at least one path that its only def is in the source node
 
 				if (res)
 				{
@@ -60,67 +59,42 @@ method finalDefSlidesOfVariable(slideDG: SlideDG, cfg: CFG, v: Variable) returns
 				}	
 		}
 	}
-
-	// foreach node - find all paths to exit (in cfg) and check if there is at least one path that it's only def is in the source node.
-	// for example: if v=i then {5,9}
-
 }
 
-method findAllPathsToExit(S: Statement, cfg: CFG, path: seq<CFGNode>, tempPathsToExit: set<seq<CFGNode>>) returns (pathsToExit: set<seq<CFGNode>>)
+method {:verify false}findAllPathsToExit(S: Statement, cfg: CFG, path: seq<CFGNode>, tempPathsToExit: set<seq<CFGNode>>) returns (pathsToExit: set<seq<CFGNode>>)
 {
+	pathsToExit := tempPathsToExit;
+	
 	match path[0] {
 		case Entry =>
 			//assert |cfg.2[path[0]]| == 1;
 			var node :| node in cfg.2[path[0]];
-			pathsToExit := findAllPathsToExit(S, cfg, [node] + path, tempPathsToExit);
+			pathsToExit := findAllPathsToExit(S, cfg, [node] + path, pathsToExit);
 		case Node(l) =>
 			var nodes := cfg.2[path[0]];
-			var cfgNode :| cfgNode in nodes;
-			nodes := nodes - {cfgNode};
 
-			match cfgNode {
-				case Entry =>
-					// Can't be.
-				case Node(l) =>
-					pathsToExit := findAllPathsToExit(S, cfg, [CFGNode.Node(l)] + path, tempPathsToExit);
-				case Exit =>
-					tempPathsToExit := tempPathsToExit + {path};
-			}
-
-			if (|cfg.2[path[0]]| == 2) // if (nodes != {})
+			while (|nodes| > 0) // Could be 1 or 2.
 			{
-				cfgNode :| cfgNode in nodes;
+				var cfgNode :| cfgNode in nodes;
 				nodes := nodes - {cfgNode};
-				//assert nodes == {};
-
-				match cfgNode {
-					case Entry =>
-						// Can't be.
-					case Node(l) =>
-						pathsToExit := findAllPathsToExit(S, cfg, [CFGNode.Node(l)] + path, tempPathsToExit);
-					case Exit =>
-						tempPathsToExit := tempPathsToExit + {path};
+				if (cfgNode !in path)
+				{
+					match cfgNode {
+						case Entry =>
+							// Can't be.
+						case Node(l) =>
+							pathsToExit := findAllPathsToExit(S, cfg, [cfgNode] + path, pathsToExit);
+						case Exit =>
+							pathsToExit := pathsToExit + {path};
+					}
 				}
-			}	
+			}
 		case Exit =>
-			tempPathsToExit := tempPathsToExit + {path};
+			pathsToExit := pathsToExit + {path};
 	}
- 
-	// אם מספר השכנים של האיבר הוא 0 אז זה exit
-	// ונכניס אותו לtempPathsToExit
-	// אם מספר השכנים הוא 1 אז נבצע אותו ונקרא רקורסיבית עם השכן שלו
-	// אם מספר השכנים הוא 2 נצבע אותו ונקרא רקורסיבית עם השכן הראשון ואז נקרא רקורסיבית עם השכן השני
-
-	// נשלח מהפונקציה הקודמת את [cfgNode]=path
-	// ואז כל פעם שנקרא רקורסיבית נוסיף את השכן לתחילת הרצף
-	// [neighbor,restOfPath]
-	// וכל פעם נעשה את הבדיקות על האיבר הראשון ברצף.
-	// ואז כל פעם שנגיע לexit
-	// נוסיף את path
-	// ל-tempPathsToExit
 }
 
-method isFinalDefSlide(pathsToExit: set<seq<CFGNode>>, vDefNode: Slide, v: Variable) returns (res: bool)
+method {:verify false}isFinalDefSlide(S: Statement, pathsToExit: set<seq<CFGNode>>, vDefNode: Slide) returns (res: bool)
 {
 	var copyPathsToExit := pathsToExit;
 	res := false;
@@ -129,13 +103,13 @@ method isFinalDefSlide(pathsToExit: set<seq<CFGNode>>, vDefNode: Slide, v: Varia
 	{
 		var pathToExit :| pathToExit in copyPathsToExit;
 		copyPathsToExit := copyPathsToExit - {pathToExit};
-		res := isDefInPath(pathToExit, vDefNode, v);
+		res := isDefInPath(S, pathToExit[..|pathToExit|-1], vDefNode);
 	}
 
 	res := !res;
 }
 
-method isDefInPath(pathToExit: seq<CFGNode>, vDefNode: Slide, v: Variable) returns (res: bool)
+method {:verify false}isDefInPath(S: Statement, pathToExit: seq<CFGNode>, vDefNode: Slide) returns (res: bool)
 {
 	//pathToExit = [cfgNode , cfgNode , ... , cfgNode]]
 	//check for each pathToExit[i] if it's def is v. If so - return true, else - return false.
@@ -143,12 +117,23 @@ method isDefInPath(pathToExit: seq<CFGNode>, vDefNode: Slide, v: Variable) retur
 	if |pathToExit| == 0 { res := false; }
 	else
 	{
-		if pathToExit[0] == vDefNode.1 { res := true; }
-		else { res := isDefInPath(pathToExit[1..], vDefNode, v); }
+		match pathToExit[0]
+		{
+			case Node(l) =>
+				var defVars := DefinedVars(S, l);
+				if (vDefNode.1 in defVars)
+				{
+					res := true;
+				}
+				else
+				{
+					res := isDefInPath(S, pathToExit[1..], vDefNode);
+				}
+		}
 	}
 }
 
-method findDefNodes(S: Statement, nodes: set<Slide>, v: Variable) returns (res: set<Slide>)
+method {:verify false}findDefNodes(S: Statement, nodes: set<Slide>, v: Variable) returns (res: set<Slide>)
 {
 	if |nodes| == 0  { res := {}; }
 	else
@@ -163,3 +148,33 @@ method findDefNodes(S: Statement, nodes: set<Slide>, v: Variable) returns (res: 
 		}
 	}
 }
+
+
+
+
+
+predicate SlideDependence(m: Slide, n: Slide, S: Statement)
+	// For n, exists n' in n.cfgNodes, this n' includes v (v is defined in m) and uses v.
+
+	//exists n' :: n' in n.2 ==> 
+
+
+function ReachingDefinitions(cfg: CFG, cfgNode: CFGNode) : set<(CFGNode, Variable)>
+	requires cfgNode in cfg.0
+	ensures forall pair :: pair in ReachingDefinitions(cfg, cfgNode) ==> DefInCFGNode(pair.0, pair.1) && SingleDefPath(cfg, cfgNode, pair.0, pair.1)
+
+
+function SlidesUseVariable(slideDG: SlideDG, slide: Slide, v: Variable) : set<Slide>
+	requires slide in slideDG.1
+	requires v == slide.1
+	ensures forall s :: s in SlidesUseVariable(slideDG, slide, v) ==> s in slideDG.1 && SlideUseVariable(s, v)
+
+
+predicate SlideUseVariable(slide: Slide, v: Variable)
+	// Check if slide uses v.
+
+predicate DefInCFGNode(cfgNode: CFGNode, v: Variable)
+	// Check if cfgNode defines v.
+
+predicate SingleDefPath(cfg: CFG, cfgNode: CFGNode, cfgNode': CFGNode, v': Variable)
+	// Check if path from cfgNode' to cfgNode exists (in cfg), that doesn't include more def to v'.
