SlideDG.dfy
@@ -8,13 +8,67 @@ type Slide = (PDGNode, Variable, set<PDGNode>)
 type Edge = (Slide, Slide, set<Variable>)
 type SlideDG = (Statement, set<Slide>, map<Slide, set<Slide>>) // map from node to it's predecssors
 
-method ComputeSlideDG(S: Statement, N: set<PDGNode>, E: set<PDGEdge>) returns (slideDG: SlideDG)
+method ComputeSlideDG(S: Statement, pdgN: set<PDGNode>, pdgE: set<PDGEdge>) returns (slideDG: SlideDG)
+{
+	var N := ComputeSlideDGNodes(S, pdgN);
+	var E := ComputeSlideDGEdges(S, N);
+	var m : map<Slide, set<Slide>>; // TODO
+
+	//slideDG := (S, N, E, m);
+}
+
+method ComputeSlideDGNodes(S: Statement, pdgN: set<PDGNode>) returns (slides: set<Slide>)
+{
+	slides := {};
+	var copyPDGN := pdgN;
+
+	while (|copyPDGN| > 0)
+	{
+		var pdgNode :| pdgNode in copyPDGN;
+		copyPDGN := copyPDGN - {pdgNode};
+		match pdgNode {
+			case Entry =>
+			case Node(l) => 
+				var subS := FindSubstatement(S, l);
+				match subS {
+					case Assignment(LHS,RHS) =>
+						var v: Variable;
+						var slide := ComputeSlide(S, v /* LHS? */, l);
+						slides := slides + {slide};
+				}
+		}
+	}
+}
+
+method ComputeSlideDGEdges(S: Statement, Slides: set<Slide>) returns (edges: set<Edge>)
+{
+	edges := {};
+	var copySlides := Slides;
+
+	while (|copySlides| > 0)
+	{
+		var Sm :| Sm in copySlides;
+		copySlides := copySlides - {Sm};		
+		var slideDepSlides := ComputeSlideDependence(Slides, Sm);
+		
+		while (|slideDepSlides| > 0)
+		{
+			var slideDep :| slideDep in slideDepSlides;
+			slideDepSlides := slideDepSlides - {slideDep};	
+			var edge := (Sm, slideDep.0, slideDep.1);
+			edges := edges + {edge};
+		}
+	}
+
+	// for each slide 
+	//		get all slide dependence slides from Slides
+	//		for each slide dependence create and label the edges
+}
+
+method ComputeSlideDependence(Slides: set<Slide>, Sm: Slide) returns (slideDepSlides: set<(Slide, set<Variable>)>)
 
 
 method ComputeSlide(S: Statement, v: Variable, l: Label) returns (n: Slide)
-
-
-
 
 
 
